New version of IndCCA.ec. Original version moved to indcca-original.

uc-dsl/examples/uc-commitment/IndCCA.ec
@@ -1,71 +1,204 @@
 (* IndCCA.ec *)
 
-(* This describes a public key encryption scheme, capturing notion of
-   IND-CCA security. *)
+(* this theory describes a public key encryption scheme capturing
+   the notion of multiple run IND-CCA security
 
-require import AllCore Distr DBool FSet.
+   it also defines a "pre-image game" along with a reduction of its
+   security to IND-CCA security *)
 
-type pkey.        (* public key *)
-type skey.        (* secret key *)
-type plaintext.   (* plain text *)
-type ciphertext.  (* cipher text *)
-type rand.        (* randomness *)
+prover quorum=2 ["Z3" "Alt-Ergo"].
 
-(* uniform, full and lossless distribution on plain texts
+require import AllCore Distr List FSet SmtMap FelTactic.
+require import StdOrder. import RealOrder.
+require import StdBigop. import Bigreal BRA.
+require import StdRing. import RField.
+require import RealSeries.
 
-   so plaintext is finite *)
+(* BEGINNING OF THEORY PARAMETERS (plus associated lemmas) *)
 
-op dplaintext : plaintext distr.
+(* the type of plain texts has pt_siz elements *)
 
-axiom dplaintext_uni : is_uniform dplaintext.
-axiom dplaintext_fu  : is_full dplaintext.
-axiom dplaintext_ll  : is_lossless dplaintext.
+type plaintext.
 
-(* uniform, full and lossless distribution on randomness
+op pt_elems : plaintext fset.  (* finite set *)
 
-   so rand is finite *)
+(* so by this axiom, pt_elems is exactly the elements of plaintext: *)
+
+axiom pt_elems (pt : plaintext) : pt \in pt_elems.
+
+op pt_siz : int = card pt_elems.
+
+op pt_def : plaintext.  (* default plain text *)
+
+lemma gt0_pt_siz : 0 < pt_siz.
+proof.
+rewrite /pt_siz ltzE /=.
+have -> : 1 = card (fset1 pt_def) by rewrite fcard1.
+rewrite subset_leq_fcard => x.
+rewrite in_fset1 => ->.
+rewrite pt_elems.
+qed.
+
+(* the type of random values has rd_siz elements *)
+
+type rand.
+
+op rd_elems : rand fset.
+
+(* so by this axiom, rd_elems is exactly the elements of rand: *)
+
+axiom rd_elems (r : rand) : r \in rd_elems.
+
+op rd_siz : int = card rd_elems.
+
+op rd_def : rand.  (* default randomness *)
+
+lemma gt0_rd_siz : 0 < rd_siz.
+proof.
+rewrite /rd_siz ltzE /=.
+have -> : 1 = card (fset1 rd_def) by rewrite fcard1.
+rewrite subset_leq_fcard => x.
+rewrite in_fset1 => ->.
+rewrite rd_elems.
+qed.
 
 op drand : rand distr.
 
-axiom drand_uni : is_uniform drand.
-axiom drand_fu  : is_full drand.
-axiom drand_ll  : is_lossless drand.
+axiom drand1E (x : rand) :
+  mu1 drand x = 1%r / rd_siz%r.
 
-(* lossless distribution on public/secret key pairs *)
+lemma drand_uni : is_uniform drand.
+proof.
+move => x y _ _.
+by rewrite 2!drand1E.
+qed.
+
+lemma drand_fu : is_full drand.
+proof.
+move => x.
+rewrite /support drand1E.
+rewrite RField.div1r invr_gt0 lt_fromint gt0_rd_siz.
+qed.
+
+lemma drand_ll : is_lossless drand.
+proof.
+have -> : drand = duniform (elems rd_elems).
+  rewrite eq_distr => x.
+  rewrite drand1E.
+  rewrite duniform1E_uniq 1:uniq_elems -memE rd_elems /=.
+  congr; by rewrite -cardE.
+rewrite duniform_ll.
+case (elems rd_elems = []) => [| //].
+move => /elems_eq_fset0 rd_elems_eq_fset0.
+have : rd_def \in fset0 by rewrite -rd_elems_eq_fset0 rd_elems.
+by rewrite in_fset0.
+qed.
+
+(* the type of cipher texts *)
+
+type ciphertext.
+
+op ct_def : ciphertext.  (* default cipher text *)
+
+(* public/secret key pairs *)
+
+type pkey.  (* public key *)
+type skey.  (* secret key *)
+
+(* lossless distribution on key pairs *)
 
 op dkeygen : (pkey * skey) distr.
 
-axiom keygen_ll : is_lossless dkeygen.
+axiom dkeygen_ll : is_lossless dkeygen.
 
 (* test if key pair is in support of dkeygen *)
 
 op valid_keys (keys : pkey * skey) : bool = support dkeygen keys.
 
-(* encrypt plaintext relative to randomness *)
+(* encrypt plain text relative to randomness *)
 
-op enc(pk : pkey, m : plaintext, r : rand) : ciphertext.
+op enc (pk : pkey, m : plaintext, r : rand) : ciphertext.
 
-(* decrypt cipher text (not needed randomness) *)
+(* decrypt cipher text (randomness not needed); returns None
+   when decryption fails, i.e., cipher text is invalid *)
 
-op dec(sk : skey, c : ciphertext) : plaintext.
+op dec (sk : skey, c : ciphertext) : plaintext option.
 
 (* correctness of encryption scheme *)
 
 axiom correctness (pk : pkey, sk : skey, m : plaintext, r : rand):
-  valid_keys (pk, sk) => dec sk (enc pk m r) = m.
+  valid_keys (pk, sk) => dec sk (enc pk m r) = Some m.
 
-(* oblivious encryption of randomness, plus inverse *)
+(* if a cipher text decrypts to a plain text, that plain text
+   encrypts to the cipher text for some randomness *)
+
+axiom dec_suceeds (pk : pkey, sk : skey, m : plaintext, c : ciphertext) :
+  valid_keys (pk, sk) => dec sk c = Some m =>
+  exists (r : rand), enc pk m r = c.
+
+(* if decrypting a cipher text fails, encryption is incapable
+   of producing the cipher text from any plain text and randomness *)
+
+lemma dec_fails (pk : pkey, sk : skey, c : ciphertext) :
+  valid_keys (pk, sk) => dec sk c = None =>
+  forall (m : plaintext, r : rand), enc pk m r <> c.
+proof.
+move => vk_pk_sk dec_sk_c_eq_None m r.
+case (enc pk m r = c) => [enc_pk_m_r_eq_c | //].
+have dec_sk_c_eq_Some_m : dec sk c = Some m.
+  by rewrite -enc_pk_m_r_eq_c correctness.
+by rewrite dec_sk_c_eq_None in dec_sk_c_eq_Some_m.
+qed.
+
+(* oblivious encryption from randomness, plus its inverse *)
 
 op obliv_enc(pk : pkey, r : rand) : ciphertext.
 op obliv_enc_inv(pk : pkey, c : ciphertext) : rand.
 
-(* obliv_enc pk is a bijection, and so rand and ciphertext have
-   the same size *)
-
-axiom obliv_enc_bij (pk : pkey, r : rand):
+axiom obliv_enc_cancel (pk : pkey, r : rand):
   obliv_enc_inv pk (obliv_enc pk r) = r.
-axiom obliv_enc_inv_bij (pk : pkey, c : ciphertext):
+
+axiom obliv_enc_inv_cancel (pk : pkey, c : ciphertext):
   obliv_enc pk (obliv_enc_inv pk c) = c.
+
+(* there is a bijection between rand and ciphertext, and so
+   they have the same number of elements *)
+
+lemma rand_ciphertext_bijective :
+  exists (f : rand -> ciphertext), bijective f.
+proof.
+have [[pk sk]] vk_pk_sk : exists (p : pkey * skey), valid_keys p.
+  have gt0_weight_dkeygen : 0%r < mu dkeygen predT by rewrite dkeygen_ll.
+  have [ex_witness _] := witness_support predT dkeygen.
+  have [x] [_ x_in_dkeygen] := ex_witness _; first rewrite gt0_weight_dkeygen.
+  by exists x.
+exists (obliv_enc pk).
+exists (obliv_enc_inv pk).
+split; [apply obliv_enc_cancel | apply obliv_enc_inv_cancel].
+qed.
+
+(* for use in the security bound of the preimage game *)
+
+op mu_obliv_enc_dec_exact (pk : pkey, sk : skey, m : plaintext) =
+  mu drand (fun r => dec sk (obliv_enc pk r) = Some m).
+
+(* TODO: can we define this in terms of pt_siz for some IND-CCA
+   schemes? *)
+
+op mu_obliv_enc_dec_exact_ub : real.
+
+axiom mu_obliv_enc_dec_exact_ub (pk : pkey, sk : skey) :
+  valid_keys (pk, sk) =>
+  mu_obliv_enc_dec_exact pk sk pt_def <= mu_obliv_enc_dec_exact_ub.
+
+(* number of allowed runs of the encryption procedure of the IND-CCA
+   oracle before a default cipher text is returned *)
+
+op runs : int.
+
+axiom ge0_runs : 0 <= runs.
+
+(* END OF THEORY PARAMETERS (and asociated lemmas) *)
 
 (* IND-CCA oracle *)
 
@@ -79,7 +212,7 @@ module type OR_INDCCA = {
   proc enc(m : plaintext) : ciphertext
 
   (* decrypt a cipher text, yielding optional plaintext that is
-     None if c was previously produced by enc, and is Some of
+     None if c was previously produced by enc, and is
      the decryption using stored secret key, otherwise *)
 
   proc dec(c : ciphertext) : plaintext option
@@ -88,19 +221,26 @@ module type OR_INDCCA = {
 (* we have two oracle implementations *)
 
 module OrIndCCA1 : OR_INDCCA = {
-  var pk : pkey
-  var sk : skey
-  var cs : ciphertext fset
+  var pk  : pkey
+  var sk  : skey
+  var cs  : ciphertext fset  (* results of encryption oracle *)
+  var ctr : int              (* runs so far *)
 
-  proc init(keys : pkey * skey) : unit = {
-    pk <- keys.`1; sk <- keys.`2; cs <- fset0;
+  proc init(pk_ : pkey, sk_ : skey) : unit = {
+    pk <- pk_; sk <- sk_; cs <- fset0; ctr <- 0;
   }
 
   proc enc(m : plaintext) : ciphertext = {
     var r : rand; var c : ciphertext;
-    r <$ drand;
-    c <- enc pk m r;  (* normal encryption *)
-    cs <- cs `|` fset1 c;
+    if (ctr < runs) {
+      r <$ drand;
+      c <- enc pk m r;  (* normal encryption *)
+      cs <- cs `|` fset1 c;
+      ctr <- ctr + 1;
+    }
+    else {
+      c <- ct_def;
+    }
     return c;
   }
 
@@ -110,26 +250,33 @@ module OrIndCCA1 : OR_INDCCA = {
       x <- None;
     }
     else {
-      x <- Some (dec sk c);  (* normal decryption *)
+      x <- dec sk c;  (* normal decryption, could be None *)
     }
     return x;
   }
 }.
 
 module OrIndCCA2 : OR_INDCCA = {
-  var pk : pkey
-  var sk : skey
-  var cs : ciphertext fset
+  var pk  : pkey
+  var sk  : skey
+  var cs  : ciphertext fset
+  var ctr : int
 
   proc init(pk_ : pkey, sk_ : skey) : unit = {
-    pk <- pk_; sk <- sk_; cs <- fset0;
+    pk <- pk_; sk <- sk_; cs <- fset0; ctr <- 0;
   }
 
   proc enc(m : plaintext) : ciphertext = {
     var r : rand; var c : ciphertext;
-    r <$ drand;
-    c <- obliv_enc pk r;  (* oblivious encryption *)
-    cs <- cs `|` fset1 c;
+    if (ctr < runs) {
+      r <$ drand;
+      c <- obliv_enc pk r;  (* oblivious encryption *)
+      cs <- cs `|` fset1 c;
+      ctr <- ctr + 1;
+    }
+    else {
+      c <- ct_def;
+    }
     return c;
   }
 
@@ -139,7 +286,7 @@ module OrIndCCA2 : OR_INDCCA = {
       x <- None;
     }
     else {
-      x <- Some (dec sk c);  (* normal decryption *)
+      x <- dec sk c;  (* normal decryption *)
     }
     return x;
   }
@@ -147,7 +294,8 @@ module OrIndCCA2 : OR_INDCCA = {
 
 (* IND-CCA adversary, parameterized by IND-CCA oracle
 
-   is given public key, and returns boolean judgment *)
+   is given public key, and returns boolean judgment;
+   it may not reinitialize oracle *)
 
 module type ADV_INDCCA (Or : OR_INDCCA) = {
   proc main(pk : pkey) : bool {Or.enc, Or.dec}
@@ -176,3 +324,608 @@ module IndCCA2 = IndCCA(OrIndCCA2).
 
    `|Pr[IndCCA1(Adv).main() @ &m : res] - Pr[IndCCA2(Adv).main() @ &m : res]|
 *)
+
+(* pre-image security *)
+
+module type OR_PI = {
+  (* initialization, given key pair *)
+
+  proc init(keys : pkey * skey) : unit
+
+  (* obliviously generate a cipher text using stored public key
+     and fresh randomness *)
+
+  proc obliv() : ciphertext
+
+  (* decrypt a cipher text, yielding optional plaintext that is None
+     if c was previously produced by obliv, and is the decryption
+     using stored secret key, otherwise *)
+
+  proc dec(c : ciphertext) : plaintext option
+
+  (* test whether enc of stored public key, x and r yields
+     one of the ciphertexts previously produced by obliv *)
+
+  proc check_preimage(x : plaintext, r : rand) : bool
+}.
+
+module OrPI : OR_PI = {
+  var pk  : pkey
+  var sk  : skey
+  var cs  : ciphertext fset
+  var ctr : int
+
+  proc init(pk_ : pkey, sk_ : skey) : unit = {
+    pk <- pk_; sk <- sk_; cs <- fset0; ctr <- 0;
+  }
+
+  proc obliv() : ciphertext = {
+    var r : rand; var c : ciphertext;
+    if (ctr < runs) {
+      r <$ drand;
+      c <- obliv_enc pk r;
+      cs <- cs `|` fset1 c;
+      ctr <- ctr + 1;
+    }
+    else {
+      c <- ct_def;
+    }
+    return c;
+  }
+
+  proc dec(c : ciphertext) : plaintext option = {
+    var x : plaintext option;
+    if (mem cs c) {
+      x <- None;
+    }
+    else {
+      x <- dec sk c;
+    }
+    return x;
+  }
+
+  proc check_preimage(x : plaintext, r : rand) : bool = {
+    return enc pk x r \in cs;
+  }
+}.
+
+module type ADV_PI (Or : OR_PI) = {
+  proc main(pk : pkey) : plaintext * rand {Or.obliv, Or.dec}
+}.
+
+module PreImage(Adv : ADV_PI) = {
+  module A = Adv(OrPI)  (* connect adversary and oracle *)
+
+  proc main() : bool = {
+    var pk : pkey; var sk : skey;
+    var x : plaintext; var r : rand;
+    var b : bool;
+    (pk, sk) <$ dkeygen;             (* generate keypair *)
+    OrPI.init(pk, sk);               (* initialize oracle *)
+    (x, r) <@ A.main(pk);            (* invoke adversary *)
+    b <@ OrPI.check_preimage(x, r);  (* see if adversary won *)
+    return b;
+  }
+}.
+
+(* construct an IND-CCA adversary from a preimage adversary;
+   for use in security upper bound *)
+
+module AdvPI2IndCCAAdv(AdvPI : ADV_PI, IndCCAOr : OR_INDCCA) = {
+  module OrPI : OR_PI = {
+    var pk  : pkey
+    var cs  : ciphertext fset
+    var ctr : int
+
+    (* sk_ won't be real, so ignore it: *)
+
+    proc init(pk_ : pkey, sk_ : skey) : unit = {
+      pk <- pk_; cs <- fset0; ctr <- 0;
+    }
+
+    proc obliv() : ciphertext = {
+      var r : rand; var c : ciphertext;
+      if (ctr < runs) {
+        c <@ IndCCAOr.enc(pt_def);  (* use IndCCAOr.enc *)
+        cs <- cs `|` fset1 c;
+        ctr <- ctr + 1;
+      }
+      else {
+        c <- ct_def;
+      }
+      return c;
+    }
+
+    proc dec(c : ciphertext) : plaintext option = {
+      var x : plaintext option;
+      x <@ IndCCAOr.dec(c);  (* use IndCCAOr.dec *)
+      return x;
+    }
+
+    proc check_preimage(x : plaintext, r : rand) : bool = {
+      return enc pk x r \in cs;
+    }
+  }
+
+  module A = AdvPI(OrPI)
+
+  proc main(pk : pkey) : bool = {
+    var b : bool; var x : plaintext; var r : rand;
+    OrPI.init(pk, witness);
+    (x, r) <@ A.main(pk);
+    b <@ OrPI.check_preimage(x, r);
+    return b /\ x <> pt_def;  (* not second conjunct *)
+  }
+}.
+
+(* start security proof *)
+
+section.
+
+declare module
+  AdvPI <: ADV_PI{-OrPI, -OrIndCCA1, -OrIndCCA2, -AdvPI2IndCCAAdv}.
+
+(* in our first step, we use up-to bad reasoning; this game
+   is like PreImage except it detects the bad event *)
+
+local module OrPI_bad1 : OR_PI = {
+  var pk  : pkey
+  var sk  : skey
+  var cs  : ciphertext fset
+  var ctr : int
+  var bad : bool
+
+  proc init(pk_ : pkey, sk_ : skey) : unit = {
+    pk <- pk_; sk <- sk_; cs <- fset0; ctr <- 0; bad <- false;
+  }
+
+  proc obliv() : ciphertext = {
+    var r : rand; var c : ciphertext;
+    if (ctr < runs) {
+      r <$ drand;
+      c <- obliv_enc pk r;
+      cs <- cs `|` fset1 c;
+      ctr <- ctr + 1;
+    }
+    else {
+      c <- ct_def;
+    }
+    return c;
+  }
+
+  proc dec(c : ciphertext) : plaintext option = {
+    var x : plaintext option;
+    if (mem cs c) {
+      x <- None;
+    }
+    else {
+      x <- dec sk c;
+    }
+    return x;
+  }
+
+  proc check_preimage(x : plaintext, r : rand) : bool = {
+    var b : bool;
+    if (enc pk x r \in cs) {
+      b <- true;
+      if (x = pt_def) {  (* bad event occurs *)
+        bad <- true;
+      }
+    }
+    else {
+      b <- false;
+    }
+    return b;
+  }
+}.
+
+local module PI_bad1 = {
+  module A = AdvPI(OrPI_bad1)
+
+  proc main() : bool = {
+    var pk : pkey; var sk : skey;
+    var x : plaintext; var r : rand;
+    var b : bool;
+    (pk, sk) <$ dkeygen;
+    OrPI_bad1.init(pk, sk);
+    (x, r) <@ A.main(pk);
+    b <@ OrPI_bad1.check_preimage(x, r);
+    return b;
+  }
+}.
+
+local lemma PreImage_AdvPI_PI_bad1 &m :
+  Pr[PreImage(AdvPI).main() @ &m : res] = Pr[PI_bad1.main() @ &m : res].
+proof.
+byequiv => //; proc.
+call (_ : ={pk, sk, cs, ctr}(OrPI, OrPI_bad1)); first auto.
+call (_ : ={pk, sk, cs, ctr}(OrPI, OrPI_bad1)); first 2 sim.
+call (_ : ={pk_, sk_} ==> ={pk, sk, cs, ctr}(OrPI, OrPI_bad1)); first sim.
+auto.
+qed.
+
+(* this game changes the result when the bad event occurs *)
+
+local module OrPI_bad2 : OR_PI = {
+  var pk  : pkey
+  var sk  : skey
+  var cs  : ciphertext fset
+  var ctr : int
+  var bad : bool
+
+  proc init(pk_ : pkey, sk_ : skey) : unit = {
+    pk <- pk_; sk <- sk_; cs <- fset0; ctr <- 0; bad <- false;
+  }
+
+  proc obliv() : ciphertext = {
+    var r : rand; var c : ciphertext;
+    if (ctr < runs) {
+      r <$ drand;
+      c <- obliv_enc pk r;
+      cs <- cs `|` fset1 c;
+      ctr <- ctr + 1;
+    }
+    else {
+      c <- ct_def;
+    }
+    return c;
+  }
+
+  proc dec(c : ciphertext) : plaintext option = {
+    var x : plaintext option;
+    if (mem cs c) {
+      x <- None;
+    }
+    else {
+      x <- dec sk c;
+    }
+    return x;
+  }
+
+  proc check_preimage(x : plaintext, r : rand) : bool = {
+    var b : bool;
+    if (enc pk x r \in cs) {
+      if (x = pt_def) {
+        b <- false;   (* we return false when normally true *)
+        bad <- true;  (* would be returned *)
+      }
+      else {
+        b <- true;
+      }
+    }
+    else {
+      b <- false;
+    }
+    return b;
+  }
+}.
+
+local module PI_bad2 = {
+  module A = AdvPI(OrPI_bad2)
+
+  proc main() : bool = {
+    var pk : pkey; var sk : skey;
+    var x : plaintext; var r : rand;
+    var b : bool;
+    (pk, sk) <$ dkeygen;
+    OrPI_bad2.init(pk, sk);
+    (x, r) <@ A.main(pk);
+    b <@ OrPI_bad2.check_preimage(x, r);
+    return b;
+  }
+}.
+
+local lemma PI_bad1_2 &m :
+  `|Pr[PI_bad1.main() @ &m : res] - Pr[PI_bad2.main() @ &m : res]| <=
+  Pr[PI_bad2.main() @ &m : OrPI_bad2.bad].
+proof.
+byequiv  (* up-to bad form of byequiv *)
+  (_ :
+   ={glob AdvPI} ==>
+   ={bad}(OrPI_bad1, OrPI_bad2) /\ (! OrPI_bad2.bad{2} => ={res})) :
+  OrPI_bad1.bad => //.
+proc.
+seq 3 3 : (={x, r} /\ ={pk, sk, cs, ctr, bad}(OrPI_bad1, OrPI_bad2)).
+call (_ : ={pk, sk, cs, ctr, bad}(OrPI_bad1, OrPI_bad2)); first 2 sim.
+call
+  (_ :
+   ={pk_, sk_} ==>
+   ={pk, sk, cs, ctr, bad}(OrPI_bad1, OrPI_bad2)); first sim.
+auto.
+inline*; auto.
+smt().
+qed.
+
+local lemma PreImage_AdvPI_PI_bad2 &m :
+  `|Pr[PreImage(AdvPI).main() @ &m : res] -
+    Pr[PI_bad2.main() @ &m : res]| <=
+  Pr[PI_bad2.main() @ &m : OrPI_bad2.bad].
+proof.
+rewrite (PreImage_AdvPI_PI_bad1 &m) (PI_bad1_2 &m).
+qed.
+
+(* for upper-bounding the probability of that bad event happening *)
+
+local module PI_bad_ub = {
+  module Or : OR_PI  = {
+    var pk  : pkey
+    var sk  : skey
+    var cs  : ciphertext fset
+    var ctr : int
+    var bad : bool
+
+    proc init(pk_ : pkey, sk_ : skey) : unit = {
+      pk <- pk_; sk <- sk_; cs <- fset0; ctr <- 0; bad <- false;
+    }
+
+    proc obliv() : ciphertext = {
+      var r : rand; var c : ciphertext;
+      if (ctr < runs) {
+        r <$ drand;
+        c <- obliv_enc pk r;
+        if (dec sk c = Some pt_def) {  (* now we set the bad event here,*)
+          bad <- true;                 (* earlier and potentially more *)
+        }                              (* often *)
+        cs <- cs `|` fset1 c;
+        ctr <- ctr + 1;
+      }
+      else {
+        c <- ct_def;
+      }
+      return c;
+    }
+
+    proc dec(c : ciphertext) : plaintext option = {
+      var x : plaintext option;
+      if (mem cs c) {
+        x <- None;
+      }
+      else {
+        x <- dec sk c;
+      }
+      return x;
+    }
+
+    (* no longer used: *)
+
+    proc check_preimage(x : plaintext, r : rand) : bool = {
+      return true;
+    }
+  }
+
+  module A = AdvPI(Or)
+
+  proc main() : bool = {
+    var pk : pkey; var sk : skey;
+    var x : plaintext; var r : rand;
+    var b : bool;
+    (pk, sk) <$ dkeygen;
+    Or.init(pk, sk);
+    (x, r) <@ A.main(pk);
+    return Or.bad;
+  }
+}.
+
+local lemma PI_bad2_ub &m :
+  Pr[PI_bad2.main() @ &m : OrPI_bad2.bad] <=
+  Pr[PI_bad_ub.main() @ &m : PI_bad_ub.Or.bad].
+proof.
+byequiv => //.
+proc.
+seq 2 2 : 
+  (={pk, sk, glob AdvPI} /\
+   ={pk, sk, cs, ctr, bad}(OrPI_bad2, PI_bad_ub.Or) /\
+   pk{1} = OrPI_bad2.pk{1} /\ sk{1} = OrPI_bad2.sk{1} /\
+   OrPI_bad2.cs{1} = fset0 /\ valid_keys (pk{1}, sk{1}) /\
+   ! OrPI_bad2.bad{1}).
+inline OrPI_bad2.init PI_bad_ub.Or.init.
+auto; smt().
+inline OrPI_bad2.check_preimage; wp => /=.
+call
+  (_ :
+   ={pk, sk, cs, ctr}(OrPI_bad2, PI_bad_ub.Or) /\
+   ! OrPI_bad2.bad{1} /\
+   ((exists c, c \in PI_bad_ub.Or.cs{2} /\
+     dec PI_bad_ub.Or.sk{2} c = Some pt_def) =>
+    PI_bad_ub.Or.bad{2})).
+proc.
+if => //.
+auto; smt(in_fsetU in_fset1).
+auto.
+proc; auto.
+auto; smt(in_fset0 correctness).
+qed.
+
+(* we use the failure event lemma to produce a concrete
+   upper bound *)
+
+local lemma PI_bad_ub_concrete &m :
+  Pr[PI_bad_ub.main() @ &m : PI_bad_ub.Or.bad] <=
+  mu_obliv_enc_dec_exact_ub * runs%r.
+proof.
+fel
+  2
+  PI_bad_ub.Or.ctr
+  (fun n => mu_obliv_enc_dec_exact_ub)
+  runs
+  PI_bad_ub.Or.bad
+  [PI_bad_ub.Or.obliv : (PI_bad_ub.Or.ctr < runs);
+   PI_bad_ub.Or.dec : false]
+  (PI_bad_ub.Or.ctr <= runs /\
+   valid_keys (PI_bad_ub.Or.pk, PI_bad_ub.Or.sk)).
+(* sum <= bound *)
+rewrite sumr_const intmulr count_predT size_range /=.
+by rewrite IntOrder.ler_maxr 1:ge0_runs.
+(* invariant good *)
+trivial.
+(* initialization *)
+inline*; auto; smt(ge0_runs).
+(* obliv bad set prob *)
+proc.
+if.
+wp.
+rnd
+  (fun r =>
+     dec PI_bad_ub.Or.sk (obliv_enc PI_bad_ub.Or.pk r) = Some pt_def).
+skip; progress.
+by apply mu_obliv_enc_dec_exact_ub.
+smt().
+auto.
+(* obliv precondition true, preservation *)
+move => c; proc.
+rcondt 1; first auto.
+auto; smt().
+(* obliv precondition false, preservation *)
+move => b c; proc.
+rcondf 1; first auto.
+auto.
+qed.
+
+local lemma PreImage_AdvPI_PI_bad2_ub &m :
+  `|Pr[PreImage(AdvPI).main() @ &m : res] -
+    Pr[PI_bad2.main() @ &m : res]| <=
+    mu_obliv_enc_dec_exact_ub * runs%r.
+proof.
+rewrite (ler_trans Pr[PI_bad2.main() @ &m : OrPI_bad2.bad]).
+rewrite (PreImage_AdvPI_PI_bad2 &m).
+rewrite (ler_trans Pr[PI_bad_ub.main() @ &m : PI_bad_ub.Or.bad]).
+rewrite (PI_bad2_ub &m).
+rewrite (PI_bad_ub_concrete &m).
+qed.
+
+local lemma PI_bad2_IndCCA2_AdvPI2IndCCAAdv_AdvPI &m :
+  Pr[PI_bad2.main() @ &m : res] =
+  Pr[IndCCA2(AdvPI2IndCCAAdv(AdvPI)).main() @ &m : res].
+proof.
+byequiv => //.
+proc.
+seq 2 2 : 
+  (={pk, sk, glob AdvPI} /\
+   ={pk, sk, cs, ctr}(OrPI_bad2, OrIndCCA2) /\
+   pk{1} = OrPI_bad2.pk{1} /\ OrPI_bad2.cs{1} = fset0 /\
+   OrPI_bad2.ctr{1} = 0).
+inline*; auto.
+inline*; wp; sp.
+call
+  (_ :
+   ={pk, cs, ctr}(OrPI_bad2, AdvPI2IndCCAAdv.OrPI) /\
+   ={pk, sk, cs, ctr}(OrPI_bad2, OrIndCCA2)).
+proc; inline*.
+if => //.
+rcondt{2} 2; first auto.
+auto.
+auto.
+proc.
+inline OrIndCCA2.dec.
+auto.
+auto.
+qed.
+
+local lemma IndCCA1_AdvPI2IndCCAAdv_AdvPI_0 &m :
+  Pr[IndCCA1(AdvPI2IndCCAAdv(AdvPI)).main() @ &m : res] = 0%r.
+proof.
+byphoare => //; proc; hoare.
+seq 2 :
+  (pk = OrIndCCA1.pk /\ sk = OrIndCCA1.sk /\ valid_keys (pk, sk) /\
+   OrIndCCA1.cs = fset0 /\ OrIndCCA1.ctr = 0).
+inline*; auto; smt().
+inline*; wp.
+seq 6 :
+  (AdvPI2IndCCAAdv.OrPI.pk = OrIndCCA1.pk /\
+   AdvPI2IndCCAAdv.OrPI.cs = OrIndCCA1.cs /\
+   AdvPI2IndCCAAdv.OrPI.ctr = OrIndCCA1.ctr /\
+   pk0 = OrIndCCA1.pk /\ valid_keys (OrIndCCA1.pk, OrIndCCA1.sk) /\
+   OrIndCCA1.ctr = 0 /\ OrIndCCA1.cs = fset0).
+auto.
+conseq
+  (_ :
+   _ ==>
+   enc AdvPI2IndCCAAdv.OrPI.pk x r \notin AdvPI2IndCCAAdv.OrPI.cs \/
+   x = pt_def).
+move => /> &hr _ cs r1 x1.
+by rewrite negb_and.
+call
+  (_ :
+   AdvPI2IndCCAAdv.OrPI.pk = OrIndCCA1.pk /\
+   AdvPI2IndCCAAdv.OrPI.cs = OrIndCCA1.cs /\
+   AdvPI2IndCCAAdv.OrPI.ctr = OrIndCCA1.ctr /\
+   valid_keys (OrIndCCA1.pk, OrIndCCA1.sk) /\
+   0 <= OrIndCCA1.ctr <= runs /\
+   (forall c,
+    c \in OrIndCCA1.cs =>
+    exists r, c = enc OrIndCCA1.pk pt_def r)).
+proc.
+if.
+wp; inline*.
+rcondt 2.
+auto.
+auto.
+move => /> &hr _ ge0_ctr _ H lt_ctr_runs r' _.
+split => [| c']; first smt().
+rewrite in_fsetU in_fset1 => [[c'_in_cs | ->]].
+by apply H.
+by exists r'.
+auto.
+proc; inline *; auto.
+auto => /> &hr vks.
+split => [| ge0_runs _].
+split => [| c']; first apply ge0_runs.
+by rewrite in_fset0.
+move => [pt' r'] cs' ctr' _ _ H /=.
+case (enc OrIndCCA1.pk{hr} pt' r' \notin cs') => [// | /= enc_pt'_r'_in_cs'].
+have [r'' enc_pt'_r'_eq_enc_pt_def_r''] :
+  exists (r'' : rand),
+  enc OrIndCCA1.pk{hr} pt' r' = enc OrIndCCA1.pk{hr} pt_def r''.
+  by apply H.
+have A :
+  dec OrIndCCA1.sk{hr} (enc OrIndCCA1.pk{hr} pt' r') = Some pt'.
+  by apply correctness.
+have B :
+  dec OrIndCCA1.sk{hr} (enc OrIndCCA1.pk{hr} pt_def r'') = Some pt_def.
+  by apply correctness.
+rewrite enc_pt'_r'_eq_enc_pt_def_r'' in A.
+by rewrite A in B.
+qed.
+
+local lemma PI_bad2_0 &m :
+  `|Pr[PI_bad2.main() @ &m : res] - 0%r| <=
+  `|Pr[IndCCA1(AdvPI2IndCCAAdv(AdvPI)).main() @ &m : res] -
+    Pr[IndCCA2(AdvPI2IndCCAAdv(AdvPI)).main() @ &m : res]|.
+proof.
+rewrite RealOrder.distrC.
+rewrite IndCCA1_AdvPI2IndCCAAdv_AdvPI_0.
+by rewrite PI_bad2_IndCCA2_AdvPI2IndCCAAdv_AdvPI.
+qed.
+
+lemma PreImage_AdvPI_sec &m :
+  Pr[PreImage(AdvPI).main() @ &m : res] <=
+  mu_obliv_enc_dec_exact_ub * runs%r +
+  `|Pr[IndCCA1(AdvPI2IndCCAAdv(AdvPI)).main() @ &m : res] -
+    Pr[IndCCA2(AdvPI2IndCCAAdv(AdvPI)).main() @ &m : res]|.
+proof.
+have -> :
+  Pr[PreImage(AdvPI).main() @ &m : res] =
+  `|Pr[PreImage(AdvPI).main() @ &m : res] - 0%r|.
+  by rewrite /= ger0_norm 1:Pr [mu_ge0].
+rewrite
+  (ler_trans
+   (`|Pr[PreImage(AdvPI).main() @ &m : res] - Pr[PI_bad2.main() @ &m : res] | +
+    `|Pr[PI_bad2.main() @ &m : res] - 0%r|)).
+rewrite ler_dist_add.
+rewrite ler_add.
+rewrite (PreImage_AdvPI_PI_bad2_ub &m).
+rewrite (PI_bad2_0 &m).
+qed.
+
+end section.
+
+lemma PreImage_AdvPI_securty
+      (AdvPI <: ADV_PI{-OrPI, -OrIndCCA1, -OrIndCCA2, -AdvPI2IndCCAAdv})
+      &m :
+  Pr[PreImage(AdvPI).main() @ &m : res] <=
+  mu_obliv_enc_dec_exact_ub * runs%r +
+  `|Pr[IndCCA1(AdvPI2IndCCAAdv(AdvPI)).main() @ &m : res] -
+    Pr[IndCCA2(AdvPI2IndCCAAdv(AdvPI)).main() @ &m : res]|.
+proof.
+apply (PreImage_AdvPI_sec AdvPI &m).
+qed.
